Pom/Lpo/Operations/Seq/Branches.lean
@@ -12,12 +12,37 @@ def ReachableWith (α : Lpofin (Label act test)) (φ : PathCond α) (x : Node) :
 def Reachable (α : Lpofin (Label act test)) : Node → Prop :=
   α.ReachableWith PathCond.empty
 
-lemma reachable_isotone [LE act] [LE test] {α β : Lpofin (Label act test)} (hle : α ≤ β)
+lemma reachable_isotone [Preorder act] [Preorder test] {α β : Lpofin (Label act test)} (hle : α ≤ β)
     {x : Node} (hx : x ∈ α.nodes) : α.Reachable x ↔ β.Reachable x := by
-  sorry
+  constructor
+  · rintro ⟨ψ, _, hform⟩
+    refine ⟨ψ.up_cast hle, bot_le, ?_⟩; exact hform.trans (le_form hle)
+  · rintro ⟨ψ, _, hform⟩
+    let ψ' : PathCond α := {
+      tests := ψ.tests ∩ α.tests
+      truth := fun ⟨z, hz⟩ ↦ ψ.truth ⟨z, Set.inter_subset_left hz⟩
+      tests_valid := Set.inter_subset_right
+    }
+    refine ⟨ψ', bot_le, ?_⟩
+    rw [← PathCond.cast_toForm (hle := hle)]; conv => rhs; exact hle.form x hx
+    refine PathCond.implies_weaken ?_ hform ?_
+    · refine ⟨Set.inter_subset_left, fun _ ↦ rfl⟩
+    · conv => arg 1; exact (hle.form x hx).symm
+      refine (α.val.property.form _ hx).1.monotone _ ?_
+      intro y hyx ⟨hyt, h⟩; refine h ⟨hyt, ?_⟩
+      obtain ⟨b, hb⟩ := (Label.isTest_iff _).mp (ψ.tests_valid hyt)
+      have hlab := le_of_le_of_eq (hle.lab y) hb
+      cases hy : α.lab y with
+      | bot => exfalso; exact α.val.property.bot y hy x hyx
+      | fork => have := le_of_eq_of_le hy.symm hlab; contradiction
+      | act a => have := le_of_eq_of_le hy.symm hlab; contradiction
+      | test t => exact (Label.isTest_iff _).mpr ⟨t, hy⟩
 
 def reachable_pred {α : Lpofin (Label act test)} {x z : Node}
-    (hr : α.Reachable x) (hz : α.rel z x) : α.Reachable z := by sorry
+    (hr : α.Reachable x) (hz : α.rel z x) : α.Reachable z := by
+  rcases hr with ⟨ψ, _, hform⟩
+  refine ⟨ψ, bot_le, ?_⟩
+  exact hform.trans ((α.val.property.form z (α.val.property.rel_dom hz).1).2 x hz)
 
 -- stuck is a path condition formula indicating that the execution will definitely
 -- encounter a ⊥ node
@@ -70,74 +95,11 @@ lemma isTest_of_le_or_bot [PartialOrder act] [PartialOrder test]
 lemma branches_monotone [PartialOrder act] [PartialOrder test]
     {α β : Lpofin (Label act test)} (hle : α ≤ β)
     {φ : PathCond α} (hφ : φ ∈ α.branches) : φ.up_cast hle ∈ β.branches := by
-  have ⟨himp, hstk, hmax⟩ := hφ
-  have ⟨v, hform⟩ := φ.sat
-  refine ⟨?_, ?_, ?_⟩
-  · intro x hx; rw [PathCond.cast_toForm]
-    exact (himp _ hx).trans <| le_form hle
-  · rw [PathCond.cast_toForm]; refine hstk.trans ?_
-    intro v h h'; apply h; exact stuck_antitone hle _ h'
-  · intro x hx htest hstk' ⟨ψ, hext, hreach⟩
-    have htest' : α.isTest x := by
-      rcases hle.succ x (tests_sub_nodes htest) with hxα | ⟨z, hz, hrel⟩
-      · cases hl : α.val.lab x <;>
-          have hlab := le_of_eq_of_le hl.symm (hle.lab x) <;> try simp at hlab
-        · exfalso; have ⟨v, hv⟩ := φ.sat
-          refine hstk _ hv ⟨⟨x, hxα, hl, ?_⟩, ?_⟩
-          · sorry
-          · conv => exact congrFun (hle.form _ hxα) _
-            sorry
-        · simp only [LE.le] at hlab; have ⟨b, h⟩ := (Label.isTest_iff _).mp htest
-          have := h.symm.trans hlab; contradiction
-        · simp only [LE.le] at hlab; have ⟨b, h⟩ := (Label.isTest_iff _).mp htest
-          conv at hlab => arg 2; exact h
-          exfalso; exact hlab
-        · exact (Label.isTest_iff _).mpr ⟨_, hl⟩
-      · sorry
-    refine hmax hx ?_ ?_ ⟨⟨ψ.tests, ψ.truth, ?_⟩, hext, ?_⟩
-    · sorry
-    · sorry
-    · sorry
-    · conv => rhs; exact hle.form _ (tests_sub_nodes htest')
-      exact hreach
+  sorry
 
 lemma le_branches [PartialOrder act] [PartialOrder test] {α β : Lpofin (Label act test)}
     (hle : α ≤ β) : α.branches = { φ | ∃ φ' ∈ β.branches, φ' = φ.up_cast hle ∧  φ.toForm ≤ α.stuck.not } := by
-  ext φ; constructor
-  · intro h; refine ⟨φ.up_cast hle, ?_, rfl, ?_⟩
-    · exact branches_monotone hle h
-    · obtain ⟨_, hstuck, _⟩ := h; exact hstuck
-  · rintro ⟨_, ⟨himp, _, hmax⟩, rfl, hstuck⟩
-    have ⟨v, hsat⟩ := φ.sat; sorry
-    -- have hsub : t ⊆ α.nodes := by
-    --   intro x hxt
-    --   have hx := tests_sub_nodes <| ht hxt
-    --   rcases hle.succ _ hx with hxα | ⟨y, hbot, hyx⟩
-    --   · exact hxα
-    --   · exfalso; refine forall_not_of_not_exists (hstuck v hsat) ⟨y, hbot⟩ ?_
-    --     refine (congrFun (hle.form y hbot.1) _).mpr ?_
-    --     refine (β.val.property.form y (hle.nodes hbot.1)).2 _ hyx v ?_
-    --     exact himp _ hsat ⟨_, hxt⟩
-    -- refine ⟨t, ?_, f, rfl, ⟨?_, hstuck⟩, ?_⟩
-    -- · intro x hx; rcases isTest_of_le_or_bot hle (ht hx) with htest | hbot
-    --   · exact htest
-    --   · exfalso
-    --     exact (hstuck v hsat) ⟨⟨x, hsub hx, hbot⟩,
-    --       (congrFun (hle.form x (hsub hx)) v).mpr (himp _ hsat ⟨x, hx⟩)⟩
-    -- · intro v hform x
-    --   exact (congrFun (hle.form x (hsub x.property)) _).mpr (himp _ hform x)
-    -- · intro x b hx htst hreach
-    --   apply hmax hx
-    --   · have ⟨c, hc⟩ := (Label.isTest_iff _).mp htst
-    --     apply (Label.isTest_iff _).mpr
-    --     obtain ⟨d, hd, _⟩ := lab_is_test_le (le_of_eq_of_le hc.symm (hle.lab x))
-    --     exact ⟨d, hd⟩
-    --   · obtain ⟨hwconj, hwstk⟩ := hreach
-    --     refine ⟨?_, ?_⟩
-    --     · intro v hform z
-    --       exact le_form hle _ (hwconj _ hform z)
-    --     · intro u hu hs
-    --       exact hwstk u hu (stuck_antitone hle u hs)
+  sorry
 
 lemma branches_not_mutually_sat {α : Lpofin (Label act test)} {φ ψ : PathCond α}
     (hφ : φ ∈ α.branches) (hψ : ψ ∈ α.branches) (hneq : φ ≠ ψ) :
